identity on rels added, further improvements

PrincipiaMetaphysicaAutomationPart1/SAVE.thy
@@ -61,9 +61,10 @@ section {* Introduction *}
    \begin{figure}[t]
   \includegraphics[height=5.5cm]{ModalRelationalTypeTheory.png}\includegraphics[height=4.5cm]{ModalRelationalTypeTheory2.png}
   \caption{Grammar of Modal Relational Type Theory. \label{mmrt}
-  Note that two kinds of (complex) formulas are introduced: ones that may have encoding subformulas and 
-  ones that don’t. The latter are designated as propositional formulas, the former ones simply as formulas. }
+  Note that two kinds of (complex) formulas are introduced: ones that may have encoding subformulas and ones that don’t.
+  The latter are designated as propositional formulas, the former ones simply as formulas. }
   \end{figure}
+
 
   To achieve this  we provide means to explicitly represents and maintain information and constraints on the 
   syntactical structure of modal relational type theory, in particular, we provide means to distinguish 
@@ -119,7 +120,7 @@ section {* Preliminaries *}
  abbreviation mkE::"'a\<Rightarrow>'a opt" ("_\<^sup>E" [109] 110)  where "\<phi>\<^sup>E \<equiv> ERR \<phi>" 
 
   text {* Some language constructs in the theory of abstract types, e.g. the actuality operator  
-  @{text "\<^bold>\<A>"} ("it is actually the case that"), refer to a (fixed) given world. To model such a 
+  @{text "\<A>"} ("it is actually the case that"), refer to a (fixed) given world. To model such a 
   global world reference we introduce a
   constant symbol (name) @{text "cw"} of world type @{text "i"}. Moreover, for technical reasons, 
   which will be clarified below, we introduce further (dummy) constant symbols for various domains. Since
@@ -135,17 +136,17 @@ section {* Embedding of Modal Relational Type Theory *}
   The language constructs of modal relational type theory are introduced step by step. 
   *}
 
-  text {* The actuality operator @{text "\<^bold>\<A>"} when applied to a formula or propositional formula 
+  text {* The actuality operator @{text "\<A>"} when applied to a formula or propositional formula 
   @{text "\<phi>"} evaluates @{text "\<phi>"} wrt the fixed given world @{text "cw"}. 
-  The compound expression @{text "\<^bold>\<A>\<phi>"} inherits its syntactical category  @{text "F"} (formula) or
+  The compound expression @{text "\<A> \<phi>"} inherits its syntactical category  @{text "F"} (formula) or
   @{text "P"} (propositional formula from @{text "\<phi>"}. If the syntactical catagory of  @{text "\<phi>"} is 
-  @{text "ERR"} (error) or @{text "T"} (term), then the syntactical catagory of @{text "\<^bold>\<A>\<phi>"} 
+  @{text "ERR"} (error) or @{text "T"} (term), then the syntactical catagory of @{text "\<A> \<phi>"} 
   is @{text "ERR"} and a dummy entity of appropriate type is returned. This illustrates the very 
   idea of our explicit structure and constraints and this scheme will repeated below
   for all the other language constructs of modal relational type theory. 
   *}
 
- abbreviation Actual::"io opt \<Rightarrow> io opt" ("\<^bold>\<A> _" [64] 65) where "\<^bold>\<A>\<phi> \<equiv> case \<phi> of 
+ abbreviation \<A>::"io opt \<Rightarrow> io opt" where "\<A> \<phi> \<equiv> case \<phi> of 
     F(\<psi>) \<Rightarrow> F(\<lambda>w. \<psi> cw) | P(\<psi>) \<Rightarrow> P(\<lambda>w. \<psi> cw) | _ \<Rightarrow> ERR(dio)"
 
   text {* 
@@ -233,7 +234,7 @@ section {* Embedding of Modal Relational Type Theory *}
 
  abbreviation lam::"(e\<Rightarrow>io opt)\<Rightarrow>(e\<Rightarrow>io) opt" (**)("\<^bold>\<lambda>")(**) where "\<^bold>\<lambda>\<Phi> \<equiv> case (\<Phi> de) of
     P(\<phi>) \<Rightarrow> T(\<lambda>x. case (\<Phi> x) of P(\<phi>) \<Rightarrow> \<phi>) | _ \<Rightarrow> ERR(\<lambda>x. dio)"
- abbreviation lamBinder::"(e\<Rightarrow>io opt)\<Rightarrow>(e\<Rightarrow>io) opt" (binder "\<^bold>\<lambda>" [8] 9)  where "\<^bold>\<lambda>x. \<phi> x \<equiv> \<^bold>\<lambda> \<phi>"
+ abbreviation lamBinder::"(e\<Rightarrow>io opt)\<Rightarrow>(e\<Rightarrow>io) opt" (binder "\<^bold>\<lambda>" [8] 9)  where "\<^bold>\<lambda> x. \<phi> x \<equiv> \<^bold>\<lambda> \<phi>"
 
  (*
  abbreviation lamtest::"(e\<Rightarrow>io opt)\<Rightarrow>(e\<Rightarrow>io) opt" (**)("lamm")(**) where "lamm \<Phi> \<equiv> case (\<Phi> de) of
@@ -252,16 +253,16 @@ section {* Embedding of Modal Relational Type Theory *}
 
   text {* 
   The Principia Metaphysica supports rigid definite descriptions. Our definition maps
-  @{text "\<^bold>\<iota>(\<lambda>x.\<phi>)"} to @{text "(THE x. \<phi> cw)"}, that is Isabelle's inbuilt description operator THE 
+  @{text "\<iota>(\<lambda>x.\<phi>)"} to @{text "(THE x. \<phi> cw)"}, that is Isabelle's inbuilt description operator THE 
   is utilized and evaluation is rigidly carried out with respect to the current world @{text "cw"}.
   Moreover, application of that is allowed only if the body of @{text "\<Phi>"}, computed by clause 
   @{text "(\<Phi> de)"}, is a propositional formula. In this case a term is returned and otherwise error 
   reported (for dummy entity @{text "de"}). We again introduce binder notation.
   *}
  
- abbreviation that::"(e\<Rightarrow>io opt)\<Rightarrow>e opt" (**)("\<^bold>\<iota>")(**)  where "\<^bold>\<iota>\<Phi> \<equiv> case (\<Phi> de) of
+ abbreviation that::"(e\<Rightarrow>io opt)\<Rightarrow>e opt" (**)("\<iota>")(**)  where "\<iota> \<Phi> \<equiv> case (\<Phi> de) of
     P(\<phi>) \<Rightarrow> T(THE x. case (\<Phi> x) of P \<psi> \<Rightarrow> \<psi> cw) | _ \<Rightarrow> ERR(de)"
- abbreviation thatBinder::"(e\<Rightarrow>io opt)\<Rightarrow>e opt" (binder "\<^bold>\<iota>" [8] 9)  where "\<^bold>\<iota>x. \<phi> x \<equiv> \<^bold>\<iota> \<phi>"
+ abbreviation thatBinder::"(e\<Rightarrow>io opt)\<Rightarrow>e opt" (binder "\<iota>" [8] 9)  where "\<iota> x. \<phi> x \<equiv> \<iota> \<phi>"
 
 
 section {* Further Logical Connectives *}
@@ -279,7 +280,7 @@ section {* Further Logical Connectives *}
  abbreviation diamond::"io opt\<Rightarrow>io opt" (**)("\<^bold>\<diamond> _" [62] 63)(**) where "\<^bold>\<diamond>\<phi> \<equiv> \<^bold>\<not>\<^bold>\<box>(\<^bold>\<not>\<phi>)"
  abbreviation exists::"('a\<Rightarrow>io opt)\<Rightarrow>io opt" (**)("\<^bold>\<exists>")(**) where "\<^bold>\<exists>\<Phi> \<equiv> case (\<Phi> da) of
     P \<phi> \<Rightarrow> P(\<lambda>w.\<exists>x. case (\<Phi> x) of P \<psi> \<Rightarrow> \<psi> w) | F \<phi> \<Rightarrow> F(\<lambda>w. \<exists>x. case (\<Phi> x) of F \<psi> \<Rightarrow> \<psi> w) | _ \<Rightarrow> ERR dio" 
- abbreviation existsBinder::"('a\<Rightarrow>io opt)\<Rightarrow>io opt" (binder "\<^bold>\<exists>" [8] 9)  where "\<^bold>\<exists>x. \<phi> x \<equiv> \<^bold>\<exists>\<phi>"
+ abbreviation existsBinder::"('a\<Rightarrow>io opt)\<Rightarrow>io opt" (binder "\<^bold>\<exists>" [8] 9)  where "\<^bold>\<exists> x. \<phi> x \<equiv> \<^bold>\<exists> \<phi>"
 
  (* abbreviation true::"io opt" (**)("\<top>\<^sup>z")(**) where "\<top>\<^sup>z \<equiv> todo; not entirely clear yet " *)
  (* abbreviation alse::"io opt" (**)("\<bottom>\<^sup>z")(**) where "\<bottom>\<^sup>z \<equiv> todo; not entirely clear yet " *)
@@ -431,217 +432,195 @@ section {* Some Basic Tests *}
   to @{text "dio\<^sup>E = X"} (simply move the curse on @{text "simp"} to see this). 
   *}
 
+ text {* Todo: ... select, adapt, and explain some of examples below ... *}
+
+lemma "\<lparr>\<^bold>\<lambda>x. \<lparr>R\<^sup>T,x\<^sup>T\<rparr> \<^bold>\<rightarrow> \<lbrace>x\<^sup>T,R\<^sup>T\<rbrace>,a\<^sup>T\<rparr> = X" apply simp oops
+
+lemma "\<exists>X. \<lparr>\<^bold>\<lambda>x. \<lparr>R\<^sup>T,x\<^sup>T\<rparr> \<^bold>\<rightarrow> \<lparr>R\<^sup>T,x\<^sup>T\<rparr>,a\<^sup>T\<rparr> = X\<^sup>P" apply simp done -- {* Solution: @{text "(\<lambda>w. True) = X"} *}
+lemma "[\<lparr>\<^bold>\<lambda>x. \<lparr>R\<^sup>T,x\<^sup>T\<rparr> \<^bold>\<rightarrow> \<lparr>R\<^sup>T,x\<^sup>T\<rparr>,a\<^sup>T\<rparr>] = \<top>" apply simp done
+
+lemma "\<lparr>\<^bold>\<lambda>x. \<lparr>R\<^sup>T,x\<^sup>T\<rparr> \<^bold>\<rightarrow> \<lparr>R\<^sup>T,x\<^sup>T\<rparr>,a\<^sup>T\<rparr> = X\<^sup>P" apply simp oops
+lemma "(\<^bold>\<lambda>x. \<lparr>R\<^sup>T,x\<^sup>T\<rparr> \<^bold>\<rightarrow> \<lbrace>x\<^sup>T,R\<^sup>T\<rbrace>) = X" apply simp oops
+
+lemma "[(\<^bold>\<forall>x. \<lparr>R\<^sup>T,x\<^sup>T\<rparr> \<^bold>\<rightarrow> \<lparr>R\<^sup>T,x\<^sup>T\<rparr>)] = \<top>" apply simp done
+lemma "[(\<^bold>\<forall>R. \<^bold>\<forall>(\<lambda>x. \<lparr>R\<^sup>T,x\<^sup>T\<rparr> \<^bold>\<rightarrow> \<lparr>R\<^sup>T,x\<^sup>T\<rparr>))] = \<top>" apply simp done
+lemma "(\<^bold>\<forall>x. \<lparr>R\<^sup>T,x\<^sup>T\<rparr> \<^bold>\<rightarrow> \<lparr>R\<^sup>T,x\<^sup>T\<rparr>) = X" apply simp oops
+
+lemma "[(\<^bold>\<forall>x. \<lbrace>x\<^sup>T,R\<^sup>T\<rbrace> \<^bold>\<rightarrow> \<lbrace>x\<^sup>T,R\<^sup>T\<rbrace>)] = \<top>" apply simp done
+lemma "(\<^bold>\<forall>x. \<lbrace>x\<^sup>T,R\<^sup>T\<rbrace> \<^bold>\<rightarrow> \<lbrace>x\<^sup>T,R\<^sup>T\<rbrace>) = X" apply simp oops
+
+lemma "[(\<^bold>\<exists>x y. \<lbrace>x\<^sup>T,R\<^sup>T\<rbrace> \<^bold>\<rightarrow> \<lbrace>y\<^sup>T,R\<^sup>T\<rbrace>)] = \<top>" apply simp done
+
+
+lemma "[(\<^bold>\<forall>x. \<lparr>R\<^sup>T,x\<^sup>T\<rparr> \<^bold>\<rightarrow> \<lbrace>x\<^sup>T,R\<^sup>T\<rbrace>)] = *" apply simp done
+lemma "[(\<^bold>\<forall>x. \<lparr>R\<^sup>T,x\<^sup>T\<rparr> \<^bold>\<rightarrow> \<lbrace>x\<^sup>T,R\<^sup>T\<rbrace>)] = X" apply simp oops
+lemma "(\<^bold>\<forall>x. \<lparr>R\<^sup>T,x\<^sup>T\<rparr> \<^bold>\<rightarrow> \<lbrace>x\<^sup>T,R\<^sup>T\<rbrace>) = X" apply simp oops
+lemma "[(\<^bold>\<forall>R. \<lparr>R\<^sup>T,x\<^sup>T\<rparr> \<^bold>\<rightarrow> \<lbrace>x\<^sup>T,R\<^sup>T\<rbrace>)] = *" apply simp done
+lemma "(\<^bold>\<forall>R. \<lparr>R\<^sup>T,x\<^sup>T\<rparr> \<^bold>\<rightarrow> \<lbrace>x\<^sup>T,R\<^sup>T\<rbrace>) = X" apply simp oops
+
+lemma "[(\<^bold>\<forall>x. \<^bold>\<exists>(\<lambda>R. \<lbrace>x\<^sup>T,R\<^sup>T\<rbrace> \<^bold>\<rightarrow> \<lbrace>x\<^sup>T,R\<^sup>T\<rbrace>))] = \<top>" apply simp done
+lemma "[(\<^bold>\<exists>x. \<^bold>\<forall>(\<lambda>R. \<lbrace>x\<^sup>T,R\<^sup>T\<rbrace> \<^bold>\<rightarrow> \<lbrace>x\<^sup>T,R\<^sup>T\<rbrace>))] = \<top>" apply simp done
+
 
  subsection {* Are Priorities Defined Correctly? *}
 
- lemma "\<phi>\<^sup>P \<^bold>\<and> \<psi>\<^sup>P \<^bold>\<rightarrow> \<chi>\<^sup>P \<equiv> (\<phi>\<^sup>P \<^bold>\<and> \<psi>\<^sup>P) \<^bold>\<rightarrow> \<chi>\<^sup>P" apply simp done
- lemma "\<phi>\<^sup>P \<^bold>\<and> \<psi>\<^sup>P \<^bold>\<rightarrow> \<chi>\<^sup>P \<equiv> \<phi>\<^sup>P \<^bold>\<and> (\<psi>\<^sup>P \<^bold>\<rightarrow> \<chi>\<^sup>P)" apply simp nitpick oops -- {* Countermodel by Nitpick *}
+lemma "\<phi>\<^sup>P \<^bold>\<and> \<psi>\<^sup>P \<^bold>\<rightarrow> \<chi>\<^sup>P \<equiv> (\<phi>\<^sup>P \<^bold>\<and> \<psi>\<^sup>P) \<^bold>\<rightarrow> \<chi>\<^sup>P" apply simp done
+lemma "\<phi>\<^sup>P \<^bold>\<and> \<psi>\<^sup>P \<^bold>\<rightarrow> \<chi>\<^sup>P \<equiv> \<phi>\<^sup>P \<^bold>\<and> (\<psi>\<^sup>P \<^bold>\<rightarrow> \<chi>\<^sup>P)" apply simp nitpick oops -- {* Countermodel by Nitpick *}
 
- lemma "(\<phi>\<^sup>P \<^bold>\<and> \<psi>\<^sup>P \<^bold>\<equiv> \<phi>\<^sup>P \<^bold>\<and> \<psi>\<^sup>P) \<equiv> ((\<phi>\<^sup>P \<^bold>\<and> \<psi>\<^sup>P) \<^bold>\<equiv> (\<phi>\<^sup>P \<^bold>\<and> \<psi>\<^sup>P))" apply simp done
- lemma "(\<phi>\<^sup>P \<^bold>\<and> \<psi>\<^sup>P \<^bold>\<equiv> \<phi>\<^sup>P \<^bold>\<and> \<psi>\<^sup>P) \<equiv> (\<phi>\<^sup>P \<^bold>\<and> (\<psi>\<^sup>P \<^bold>\<equiv> \<phi>\<^sup>P) \<^bold>\<and> \<psi>\<^sup>P)" apply simp nitpick oops -- {* Countermodel by Nitpick *}
+lemma "(\<phi>\<^sup>P \<^bold>\<and> \<psi>\<^sup>P \<^bold>\<equiv> \<phi>\<^sup>P \<^bold>\<and> \<psi>\<^sup>P) \<equiv> ((\<phi>\<^sup>P \<^bold>\<and> \<psi>\<^sup>P) \<^bold>\<equiv> (\<phi>\<^sup>P \<^bold>\<and> \<psi>\<^sup>P))" apply simp done
+lemma "(\<phi>\<^sup>P \<^bold>\<and> \<psi>\<^sup>P \<^bold>\<equiv> \<phi>\<^sup>P \<^bold>\<and> \<psi>\<^sup>P) \<equiv> (\<phi>\<^sup>P \<^bold>\<and> (\<psi>\<^sup>P \<^bold>\<equiv> \<phi>\<^sup>P) \<^bold>\<and> \<psi>\<^sup>P)" apply simp nitpick oops -- {* Countermodel by Nitpick *}
 
 
 section {* E!, O!, A! and =E *}
 
-  text {* 
-  We introduce the distinguished 1-place relation constant: E (read: ‘being concrete’ or ‘concreteness’) 
-  *}
+ text {* We introduce the distinguished 1-place relation constant: E (read: ‘being concrete’ or ‘concreteness’) *}
 
- consts E::"(e\<Rightarrow>io)"
+consts E::"(e\<Rightarrow>io)"
  
-  text {* 
-  Being ordinary is defined as being possibly concrete. 
-  *}
+ text {* Being ordinary is defined as being possibly concrete. *}
 
- abbreviation ordinaryObject::"(e\<Rightarrow>io) opt" (**)("O!")(**) where "O! \<equiv> \<^bold>\<lambda>x. \<^bold>\<diamond>\<lparr>E\<^sup>T,x\<^sup>T\<rparr>"
+abbreviation ordinaryObject::"(e\<Rightarrow>io) opt" (**)("O!")(**) where "O! \<equiv> \<^bold>\<lambda>x. \<^bold>\<diamond>\<lparr>E\<^sup>T,x\<^sup>T\<rparr>"
 
- lemma "O! = X" apply simp oops       -- {* X is (\<lambda>x w. Ex (E x))\<^sup>T *}
+lemma "O! = X" apply simp oops       -- {* X is (\<lambda>x w. Ex (E x))\<^sup>T *}
 
-  text {* 
-  Being abstract is is defined as not possibly being concrete. 
-  *}
+ text {* Being abstract is is defined as not possibly being concrete. *}
 
- abbreviation abstractObject::"(e\<Rightarrow>io) opt" (**)("A!")(**) where "A! \<equiv> \<^bold>\<lambda>x. \<^bold>\<not>(\<^bold>\<diamond>\<lparr>E\<^sup>T,x\<^sup>T\<rparr>)"
+abbreviation abstractObject::"(e\<Rightarrow>io) opt" (**)("A!")(**) where "A! \<equiv> \<^bold>\<lambda>x. \<^bold>\<not>(\<^bold>\<diamond>\<lparr>E\<^sup>T,x\<^sup>T\<rparr>)"
 
- lemma "A! = X" apply simp oops       -- {* X is  (\<lambda>x w. \<forall>xa. \<not> E x xa)\<^sup>T *}
+lemma "A! = X" apply simp oops       -- {* X is  (\<lambda>x w. \<forall>xa. \<not> E x xa)\<^sup>T *}
 
-
-  text {* 
-  Identity relations @{text "\<^bold>=\<^sub>E"} and @{text "\<^bold>="} are introduced. 
-  *}
-
- abbreviation identityE::"e opt\<Rightarrow>e opt\<Rightarrow>io opt" (**)(infixl "\<^bold>=\<^sub>E" 63)(**) where "x \<^bold>=\<^sub>E y \<equiv> 
-    \<lparr>O!,x\<rparr> \<^bold>\<and> \<lparr>O!,y\<rparr> \<^bold>\<and> \<^bold>\<box>(\<^bold>\<forall>F. \<lparr>F\<^sup>T,x\<rparr> \<^bold>\<equiv> \<lparr>F\<^sup>T,y\<rparr>)"
-
- lemma "a\<^sup>T \<^bold>=\<^sub>E a\<^sup>T = X" apply simp oops      -- {* X is (\<lambda>w. \<exists>x. E a x)\<^sup>P *}
-
-
- subsection {* Identity on Individuals *}
-
- abbreviation identityI::"e opt\<Rightarrow>e opt\<Rightarrow>io opt" (**)(infixl "\<^bold>=" 63)(**) where "x \<^bold>= y \<equiv> 
-    x \<^bold>=\<^sub>E y \<^bold>\<or> (\<lparr>A!,x\<rparr> \<^bold>\<and> \<lparr>A!,y\<rparr> \<^bold>\<and> \<^bold>\<box>(\<^bold>\<forall>F. \<lbrace>x,F\<^sup>T\<rbrace> \<^bold>\<equiv> \<lbrace>y,F\<^sup>T\<rbrace>))"
-  
- text {* 
- Problem!?: @{text "a\<^sup>T \<^bold>= a\<^sup>T"} is neither a formula nor a propositional formula 
+ text {* Identity relations @{text "\<^bold>=\<^sub>E"} and @{text "\<^bold>="} are introduced. 
  *}
 
- lemma "a\<^sup>T \<^bold>= a\<^sup>T = X" apply simp oops                                        -- {* X is dio\<^sup>E *}
- lemma "(\<lparr>A!,a\<^sup>T\<rparr> \<^bold>\<and> \<lparr>A!,a\<^sup>T\<rparr> \<^bold>\<and> \<^bold>\<box>(\<^bold>\<forall>F. \<lbrace>a\<^sup>T,F\<^sup>T\<rbrace> \<^bold>\<equiv> \<lbrace>a\<^sup>T,F\<^sup>T\<rbrace>)) = X" apply simp oops   -- {* X is dio\<^sup>E *}
- lemma "(\<lparr>A!,a\<^sup>T\<rparr> \<^bold>\<and> \<lparr>A!,a\<^sup>T\<rparr>) = X" apply simp oops                             -- {* X is (\<lambda>w. \<forall>x. \<not> E a x)\<^sup>P *}
- lemma "\<^bold>\<box>(\<^bold>\<forall>F. \<lbrace>a\<^sup>T,F\<^sup>T\<rbrace> \<^bold>\<equiv> \<lbrace>a\<^sup>T,F\<^sup>T\<rbrace>) = X" apply simp oops                       -- {* X is (\<lambda>w. True)\<^sup>F *}
+
+(* 
+abbreviation identitye::"(e\<Rightarrow>e\<Rightarrow>io) opt" (**)("\<^bold>=\<^sub>e")(**) where "\<^bold>=\<^sub>e \<equiv> 
+  \<^bold>\<lambda>\<^sup>2(\<lambda>x y. \<lparr>O!,x\<^sup>T\<rparr> \<^bold>\<and> \<lparr>O!,y\<^sup>T\<rparr> \<^bold>\<and> \<^bold>\<box>(\<^bold>\<forall>F. \<lparr>F\<^sup>T,x\<^sup>T\<rparr> \<^bold>\<equiv> \<lparr>F\<^sup>T,y\<^sup>T\<rparr>))"
+abbreviation identityE::"e opt\<Rightarrow>e opt\<Rightarrow>io opt" (**)(infixl "\<^bold>=\<^sub>E" 63)(**) where "x \<^bold>=\<^sub>E y \<equiv> \<lparr>\<^bold>=\<^sub>e,x,y\<rparr>"
+*)
+
+abbreviation identityE::"e opt\<Rightarrow>e opt\<Rightarrow>io opt" (**)(infixl "\<^bold>=\<^sub>E" 63)(**) 
+  where "x \<^bold>=\<^sub>E y \<equiv> \<lparr>O!,x\<rparr> \<^bold>\<and> \<lparr>O!,y\<rparr> \<^bold>\<and> \<^bold>\<box>(\<^bold>\<forall>F. \<lparr>F\<^sup>T,x\<rparr> \<^bold>\<equiv> \<lparr>F\<^sup>T,y\<rparr>)"
+
+lemma "a\<^sup>T \<^bold>=\<^sub>E a\<^sup>T = X" apply simp oops      -- {* X is (\<lambda>w. \<exists>x. E a x)\<^sup>P *}
+
+subsection {* Identity on Individuals *}
+
+abbreviation identityI::"e opt\<Rightarrow>e opt\<Rightarrow>io opt" (**)(infixl "\<^bold>=" 63)(**) 
+  where "x \<^bold>= y \<equiv> x \<^bold>=\<^sub>E y \<^bold>\<or> (\<lparr>A!,x\<rparr> \<^bold>\<and> \<lparr>A!,y\<rparr> \<^bold>\<and> \<^bold>\<box>(\<^bold>\<forall>F. \<lbrace>x,F\<^sup>T\<rbrace> \<^bold>\<equiv> \<lbrace>y,F\<^sup>T\<rbrace>))"
+  
+ text {* Problem!?: @{text "a\<^sup>T \<^bold>= a\<^sup>T"} is neither a formula nor a propositional formula *}
+
+lemma "a\<^sup>T \<^bold>= a\<^sup>T = X" apply simp oops                                        -- {* X is dio\<^sup>E *}
+lemma "(\<lparr>A!,a\<^sup>T\<rparr> \<^bold>\<and> \<lparr>A!,a\<^sup>T\<rparr> \<^bold>\<and> \<^bold>\<box>(\<^bold>\<forall>F. \<lbrace>a\<^sup>T,F\<^sup>T\<rbrace> \<^bold>\<equiv> \<lbrace>a\<^sup>T,F\<^sup>T\<rbrace>)) = X" apply simp oops   -- {* X is dio\<^sup>E *}
+lemma "(\<lparr>A!,a\<^sup>T\<rparr> \<^bold>\<and> \<lparr>A!,a\<^sup>T\<rparr>) = X" apply simp oops                             -- {* X is (\<lambda>w. \<forall>x. \<not> E a x)\<^sup>P *}
+lemma "\<^bold>\<box>(\<^bold>\<forall>F. \<lbrace>a\<^sup>T,F\<^sup>T\<rbrace> \<^bold>\<equiv> \<lbrace>a\<^sup>T,F\<^sup>T\<rbrace>) = X" apply simp oops                       -- {* X is (\<lambda>w. True)\<^sup>F *}
 
 
- subsection {* Identitiy on Relations *}
+subsection {* Identitiy on Relations *}
 
- abbreviation identityRel1::" ((e\<Rightarrow>io) opt)\<Rightarrow>((e\<Rightarrow>io) opt)\<Rightarrow>io opt" (**)(infixl "\<^bold>=\<^sup>1" 63)(**) 
-   where "F1 \<^bold>=\<^sup>1 G1 \<equiv> \<^bold>\<box>(\<^bold>\<forall>x. \<lbrace>x\<^sup>T,F1\<rbrace> \<^bold>\<equiv> \<lbrace>x\<^sup>T,G1\<rbrace>)"
+abbreviation equalityRel1::" ((e\<Rightarrow>io) opt)\<Rightarrow>((e\<Rightarrow>io) opt)\<Rightarrow>io opt" (**)(infixl "\<^bold>=\<^sup>1" 63)(**) 
+ where "F1 \<^bold>=\<^sup>1 G1 \<equiv> \<^bold>\<box>(\<^bold>\<forall>x. \<lbrace>x\<^sup>T,F1\<rbrace> \<^bold>\<equiv> \<lbrace>x\<^sup>T,G1\<rbrace>)"
 
- abbreviation identityRel2::" ((e\<Rightarrow>e\<Rightarrow>io) opt)\<Rightarrow>((e\<Rightarrow>e\<Rightarrow>io) opt)\<Rightarrow>io opt" (**)(infixl "\<^bold>=\<^sup>2" 63)(**) 
-   where "F2 \<^bold>=\<^sup>2 G2 \<equiv> \<^bold>\<forall>x1.(  (\<^bold>\<lambda>y.\<lparr>F2,y\<^sup>T,x1\<^sup>T\<rparr>) \<^bold>=\<^sup>1 (\<^bold>\<lambda>y.\<lparr>G2,y\<^sup>T,x1\<^sup>T\<rparr>)
-                          \<^bold>\<and> (\<^bold>\<lambda>y.\<lparr>F2,x1\<^sup>T,y\<^sup>T\<rparr>) \<^bold>=\<^sup>1 (\<^bold>\<lambda>y.\<lparr>G2,x1\<^sup>T,y\<^sup>T\<rparr>))"
+abbreviation equalityRel2::" ((e\<Rightarrow>e\<Rightarrow>io) opt)\<Rightarrow>((e\<Rightarrow>e\<Rightarrow>io) opt)\<Rightarrow>io opt" (**)(infixl "\<^bold>=\<^sup>1" 63)(**) 
+ where "F2 \<^bold>=\<^sup>2 G2 \<equiv> \<^bold>\<forall> x. ("
 
- abbreviation identityRel3::" ((e\<Rightarrow>e\<Rightarrow>e\<Rightarrow>io) opt)\<Rightarrow>((e\<Rightarrow>e\<Rightarrow>e\<Rightarrow>io) opt)\<Rightarrow>io opt" (**)(infixl "\<^bold>=\<^sup>3" 63)(**) 
-   where "F3 \<^bold>=\<^sup>3 G3 \<equiv> \<^bold>\<forall>x1 x2.(  (\<^bold>\<lambda>y.\<lparr>F3,y\<^sup>T,x1\<^sup>T,x2\<^sup>T\<rparr>) \<^bold>=\<^sup>1 (\<^bold>\<lambda>y.\<lparr>G3,y\<^sup>T,x1\<^sup>T,x2\<^sup>T\<rparr>)
-                             \<^bold>\<and> (\<^bold>\<lambda>y.\<lparr>F3,x1\<^sup>T,y\<^sup>T,x2\<^sup>T\<rparr>) \<^bold>=\<^sup>1 (\<^bold>\<lambda>y.\<lparr>G3,x1\<^sup>T,y\<^sup>T,x2\<^sup>T\<rparr>)
-                             \<^bold>\<and> (\<^bold>\<lambda>y.\<lparr>F3,x1\<^sup>T,x2\<^sup>T,y\<^sup>T\<rparr>) \<^bold>=\<^sup>1 (\<^bold>\<lambda>y.\<lparr>G3,x1\<^sup>T,x2\<^sup>T,y\<^sup>T\<rparr>))"
+lemma "a\<^sup>T \<^bold>= a\<^sup>T = X" apply simp oops   
 
- lemma "F1\<^sup>T \<^bold>=\<^sup>1 G1\<^sup>T = X" apply simp oops -- {* X is (\<lambda>w. \<forall>w x. (F1 x w \<longrightarrow> G1 x w) \<and> (G1 x w \<longrightarrow> F1 x w))\<^sup>F *}
- lemma "F2\<^sup>T \<^bold>=\<^sup>2 G2\<^sup>T = X" apply simp oops -- {* X is (...)\<^sup>F *} 
- lemma "F3\<^sup>T \<^bold>=\<^sup>3 G3\<^sup>T = X" apply simp oops -- {* X is (...)\<^sup>F *}   
- lemma "\<lbrace>x\<^sup>T,F1\<^sup>T\<rbrace> \<^bold>\<equiv> \<lbrace>x\<^sup>T,G1\<^sup>T\<rbrace> = X" apply simp oops -- {* X is (...)\<^sup>F *}   
- lemma "\<lparr>F1\<^sup>T,x\<^sup>T\<rparr> \<^bold>\<equiv> \<lparr>G1\<^sup>T,x\<^sup>T\<rparr> = X" apply simp oops -- {* X is (...)\<^sup>P *}   
- lemma "(\<^bold>\<lambda>y.\<lparr>F2\<^sup>T,y\<^sup>T,x1\<^sup>T\<rparr>)= X" apply simp oops -- {* X is (...)\<^sup>T *}  
-
- abbreviation equalityRel0::"io opt\<Rightarrow>io opt\<Rightarrow>io opt" (**)(infixl "\<^bold>=\<^sup>0" 63)(**) 
-   where "F0 \<^bold>=\<^sup>0 G0 \<equiv> (\<^bold>\<lambda>y . F0) \<^bold>=\<^sup>1 (\<^bold>\<lambda>y. G0)"
+abbreviation equalityRel0::"io opt\<Rightarrow>io opt\<Rightarrow>io opt" (**)(infixl "\<^bold>=\<^sup>0" 63)(**) 
+ where "F0 \<^bold>=\<^sup>0 G0 \<equiv> (\<^bold>\<lambda>y . F0) \<^bold>=\<^sup>1 (\<^bold>\<lambda>y. G0)"
 
 
-  text {* 
-  Some tests: 
-  *}
 
- lemma "[a\<^sup>T \<^bold>=\<^sub>E a\<^sup>T] = \<top>" apply simp nitpick oops -- {* Countermodel by Nitpick *}
- lemma "[\<lparr>O!,a\<^sup>T\<rparr> \<^bold>\<rightarrow> a\<^sup>T \<^bold>=\<^sub>E a\<^sup>T] = \<top>" apply simp done
 
- lemma "[(\<^bold>\<forall>F. \<lparr>F\<^sup>T,x\<^sup>T\<rparr> \<^bold>\<equiv> \<lparr>F\<^sup>T,x\<^sup>T\<rparr>)] = \<top>" apply simp done
- lemma "[\<lparr>O!,a\<^sup>T\<rparr> \<^bold>\<rightarrow> \<lparr>\<^bold>\<lambda>x. x\<^sup>T \<^bold>=\<^sub>E a\<^sup>T,a\<^sup>T\<rparr>] = \<top>" apply simp done
 
- lemma "[(\<^bold>\<exists>F. \<lbrace>a\<^sup>T,F\<^sup>T\<rbrace>)] = \<top>" apply simp by auto
+subsection {* Further Test Examples *}
 
- lemma "[(\<^bold>\<exists>\<phi>. \<phi>\<^sup>P)] = \<top>" apply simp by auto
- lemma "[(\<^bold>\<exists>\<phi>. \<phi>\<^sup>F)] = \<top>" apply simp by auto
+ text {* Todo: ... select, adapt, and explain some of examples below *}
+
+lemma "[a\<^sup>T \<^bold>=\<^sub>E a\<^sup>T] = \<top>" apply simp nitpick oops -- {* Countermodel by Nitpick *}
+
+lemma "[\<lparr>O!,a\<^sup>T\<rparr> \<^bold>\<rightarrow> a\<^sup>T \<^bold>=\<^sub>E a\<^sup>T] = \<top>" apply simp done
+
+lemma "[(\<^bold>\<forall>F. \<lparr>F\<^sup>T,x\<^sup>T\<rparr> \<^bold>\<equiv> \<lparr>F\<^sup>T,x\<^sup>T\<rparr>)] = \<top>" apply simp done
+lemma "[\<lparr>O!,a\<^sup>T\<rparr> \<^bold>\<rightarrow> \<lparr>\<^bold>\<lambda>x. x\<^sup>T \<^bold>=\<^sub>E a\<^sup>T,a\<^sup>T\<rparr>] = \<top>" apply simp done
+
+lemma "[(\<^bold>\<exists>F. \<lbrace>a\<^sup>T,F\<^sup>T\<rbrace>)] = \<top>" apply simp by auto
+
+lemma "[(\<^bold>\<exists>\<phi>. \<phi>\<^sup>P)] = \<top>" apply simp by auto
+lemma "[(\<^bold>\<exists>\<phi>. \<phi>\<^sup>F)] = \<top>" apply simp by auto
 
 
 section {* Axioms *}
 
- subsection {* Axioms for Negations and Conditionals *}
+subsection {* Axioms for Negations and Conditionals *}
 
- lemma a21_1_P: "[\<phi>\<^sup>P \<^bold>\<rightarrow> (\<phi>\<^sup>P \<^bold>\<rightarrow> \<phi>\<^sup>P)] = \<top>" apply simp done
- lemma a21_1_F: "[\<phi>\<^sup>F \<^bold>\<rightarrow> (\<phi>\<^sup>F \<^bold>\<rightarrow> \<phi>\<^sup>F)] = \<top>" apply simp done
- lemma a21_2_P: "[(\<phi>\<^sup>P \<^bold>\<rightarrow> (\<psi>\<^sup>P \<^bold>\<rightarrow> \<chi>\<^sup>P)) \<^bold>\<rightarrow> ((\<phi>\<^sup>P \<^bold>\<rightarrow> \<psi>\<^sup>P) \<^bold>\<rightarrow> (\<phi>\<^sup>P \<^bold>\<rightarrow> \<chi>\<^sup>P))] = \<top>" apply simp done
- lemma a21_2_F: "[(\<phi>\<^sup>F \<^bold>\<rightarrow> (\<psi>\<^sup>F \<^bold>\<rightarrow> \<chi>\<^sup>F)) \<^bold>\<rightarrow> ((\<phi>\<^sup>F \<^bold>\<rightarrow> \<psi>\<^sup>F) \<^bold>\<rightarrow> (\<phi>\<^sup>F \<^bold>\<rightarrow> \<chi>\<^sup>F))] = \<top>" apply simp done
- lemma a21_3_P: "[(\<^bold>\<not>\<phi>\<^sup>P \<^bold>\<rightarrow> \<^bold>\<not>\<psi>\<^sup>P) \<^bold>\<rightarrow> ((\<^bold>\<not>\<phi>\<^sup>P \<^bold>\<rightarrow> \<psi>\<^sup>P) \<^bold>\<rightarrow> \<phi>\<^sup>P)] = \<top>" apply simp done
- lemma a21_3_F: "[(\<^bold>\<not>\<phi>\<^sup>F \<^bold>\<rightarrow> \<^bold>\<not>\<psi>\<^sup>F) \<^bold>\<rightarrow> ((\<^bold>\<not>\<phi>\<^sup>F \<^bold>\<rightarrow> \<psi>\<^sup>F) \<^bold>\<rightarrow> \<phi>\<^sup>F)] = \<top>" apply simp done
+lemma a21_1_P: "[\<phi>\<^sup>P \<^bold>\<rightarrow> (\<phi>\<^sup>P \<^bold>\<rightarrow> \<phi>\<^sup>P)] = \<top>" apply simp done
+lemma a21_1_F: "[\<phi>\<^sup>F \<^bold>\<rightarrow> (\<phi>\<^sup>F \<^bold>\<rightarrow> \<phi>\<^sup>F)] = \<top>" apply simp done
+lemma a21_2_P: "[(\<phi>\<^sup>P \<^bold>\<rightarrow> (\<psi>\<^sup>P \<^bold>\<rightarrow> \<chi>\<^sup>P)) \<^bold>\<rightarrow> ((\<phi>\<^sup>P \<^bold>\<rightarrow> \<psi>\<^sup>P) \<^bold>\<rightarrow> (\<phi>\<^sup>P \<^bold>\<rightarrow> \<chi>\<^sup>P))] = \<top>" apply simp done
+lemma a21_2_F: "[(\<phi>\<^sup>F \<^bold>\<rightarrow> (\<psi>\<^sup>F \<^bold>\<rightarrow> \<chi>\<^sup>F)) \<^bold>\<rightarrow> ((\<phi>\<^sup>F \<^bold>\<rightarrow> \<psi>\<^sup>F) \<^bold>\<rightarrow> (\<phi>\<^sup>F \<^bold>\<rightarrow> \<chi>\<^sup>F))] = \<top>" apply simp done
+lemma a21_3_P: "[(\<^bold>\<not>\<phi>\<^sup>P \<^bold>\<rightarrow> \<^bold>\<not>\<psi>\<^sup>P) \<^bold>\<rightarrow> ((\<^bold>\<not>\<phi>\<^sup>P \<^bold>\<rightarrow> \<psi>\<^sup>P) \<^bold>\<rightarrow> \<phi>\<^sup>P)] = \<top>" apply simp done
+lemma a21_3_F: "[(\<^bold>\<not>\<phi>\<^sup>F \<^bold>\<rightarrow> \<^bold>\<not>\<psi>\<^sup>F) \<^bold>\<rightarrow> ((\<^bold>\<not>\<phi>\<^sup>F \<^bold>\<rightarrow> \<psi>\<^sup>F) \<^bold>\<rightarrow> \<phi>\<^sup>F)] = \<top>" apply simp done
 
- subsection {* Axioms of Identity *}
-  text {* todo *}
+subsection {* Axioms of Identity *}
+text {* todo *}
 
- subsection {* Axioms of Quantification *}
-  text {* todo *}
+subsection {* Axioms of Quantification *}
+text {* todo *}
 
- subsection {* Axioms of Actuality *}
+subsection {* Axioms of Actuality *}
 
- lemma a31_1_P: "[\<^bold>\<A>(\<^bold>\<not>\<phi>\<^sup>P) \<^bold>\<equiv> \<^bold>\<not>\<^bold>\<A>(\<phi>\<^sup>P)] = \<top>" apply simp done
- lemma a31_1_F: "[\<^bold>\<A>(\<^bold>\<not>\<phi>\<^sup>F) \<^bold>\<equiv> \<^bold>\<not>\<^bold>\<A>(\<phi>\<^sup>F)] = \<top>" apply simp done
- lemma a31_2_P: "[\<^bold>\<A>(\<phi>\<^sup>P \<^bold>\<rightarrow> \<psi>\<^sup>P) \<^bold>\<equiv> (\<^bold>\<A>(\<phi>\<^sup>P) \<^bold>\<rightarrow> \<^bold>\<A>(\<psi>\<^sup>P))] = \<top>" apply simp done
- lemma a31_2_F: "[\<^bold>\<A>(\<phi>\<^sup>F \<^bold>\<rightarrow> \<psi>\<^sup>F) \<^bold>\<equiv> (\<^bold>\<A>(\<phi>\<^sup>F) \<^bold>\<rightarrow> \<^bold>\<A>(\<psi>\<^sup>F))] = \<top>" apply simp done
- lemma a31_3_P: "[\<^bold>\<A>(\<^bold>\<forall>x. \<phi>\<^sup>P) \<^bold>\<equiv> (\<^bold>\<forall>x. \<^bold>\<A>(\<phi>\<^sup>P))] = \<top>" apply simp done
- lemma a31_3_F: "[(\<^bold>\<A>(\<^bold>\<forall>x. \<phi>\<^sup>F) \<^bold>\<equiv> (\<^bold>\<forall>x. \<^bold>\<A>(\<phi>\<^sup>F)))] = \<top>" apply simp done
- lemma a31_4_P: "[\<^bold>\<A>(\<phi>\<^sup>P) \<^bold>\<equiv> \<^bold>\<A>(\<^bold>\<A>(\<phi>\<^sup>P))] = \<top>" apply simp done
- lemma a31_4_F: "[\<^bold>\<A>(\<phi>\<^sup>F) \<^bold>\<equiv> \<^bold>\<A>(\<^bold>\<A>(\<phi>\<^sup>F))] = \<top>" apply simp done
+lemma a31_1_P: "[\<A>(\<^bold>\<not>\<phi>\<^sup>P) \<^bold>\<equiv> \<^bold>\<not>\<A>(\<phi>\<^sup>P)] = \<top>" apply simp done
+lemma a31_1_F: "[\<A>(\<^bold>\<not>\<phi>\<^sup>F) \<^bold>\<equiv> \<^bold>\<not>\<A>(\<phi>\<^sup>F)] = \<top>" apply simp done
+lemma a31_2_P: "[\<A>(\<phi>\<^sup>P \<^bold>\<rightarrow> \<psi>\<^sup>P) \<^bold>\<equiv> (\<A>(\<phi>\<^sup>P) \<^bold>\<rightarrow> \<A>(\<psi>\<^sup>P))] = \<top>" apply simp done
+lemma a31_2_F: "[\<A>(\<phi>\<^sup>F \<^bold>\<rightarrow> \<psi>\<^sup>F) \<^bold>\<equiv> (\<A>(\<phi>\<^sup>F) \<^bold>\<rightarrow> \<A>(\<psi>\<^sup>F))] = \<top>" apply simp done
+lemma a31_3_P: "[\<A>(\<^bold>\<forall>x. \<phi>\<^sup>P) \<^bold>\<equiv> (\<^bold>\<forall>x. \<A>(\<phi>\<^sup>P))] = \<top>" apply simp done
+lemma a31_3_F: "[(\<A>(\<^bold>\<forall>x. \<phi>\<^sup>F) \<^bold>\<equiv> (\<^bold>\<forall>x. \<A>(\<phi>\<^sup>F)))] = \<top>" apply simp done
+lemma a31_4_P: "[\<A>(\<phi>\<^sup>P) \<^bold>\<equiv> \<A>(\<A>(\<phi>\<^sup>P))] = \<top>" apply simp done
+lemma a31_4_F: "[\<A>(\<phi>\<^sup>F) \<^bold>\<equiv> \<A>(\<A>(\<phi>\<^sup>F))] = \<top>" apply simp done
 
- subsection {* Axioms of Necessity *}
+subsection {* Axioms of Necessity *}
 
- lemma a32_1_P: "[(\<^bold>\<box>(\<phi>\<^sup>P \<^bold>\<rightarrow> \<phi>\<^sup>P)) \<^bold>\<rightarrow> (\<^bold>\<box>\<phi>\<^sup>P \<^bold>\<rightarrow> \<^bold>\<box>\<phi>\<^sup>P)] = \<top>" apply simp done     (* K Schema *)
- lemma a32_1_F: "[(\<^bold>\<box>(\<phi>\<^sup>F \<^bold>\<rightarrow> \<phi>\<^sup>F)) \<^bold>\<rightarrow> (\<^bold>\<box>\<phi>\<^sup>F \<^bold>\<rightarrow> \<^bold>\<box>\<phi>\<^sup>F)] = \<top>" apply simp done     (* K Schema *)
- lemma a32_2_P: "[\<^bold>\<box>\<phi>\<^sup>P \<^bold>\<rightarrow> \<phi>\<^sup>P] = \<top>" apply simp done                           (* T Schema *)
- lemma a32_2_F: "[\<^bold>\<box>\<phi>\<^sup>F \<^bold>\<rightarrow> \<phi>\<^sup>F] = \<top>" apply simp done                           (* T Schema *)
+lemma a32_1_P: "[(\<^bold>\<box>(\<phi>\<^sup>P \<^bold>\<rightarrow> \<phi>\<^sup>P)) \<^bold>\<rightarrow> (\<^bold>\<box>\<phi>\<^sup>P \<^bold>\<rightarrow> \<^bold>\<box>\<phi>\<^sup>P)] = \<top>" apply simp done     (* K Schema *)
+lemma a32_1_F: "[(\<^bold>\<box>(\<phi>\<^sup>F \<^bold>\<rightarrow> \<phi>\<^sup>F)) \<^bold>\<rightarrow> (\<^bold>\<box>\<phi>\<^sup>F \<^bold>\<rightarrow> \<^bold>\<box>\<phi>\<^sup>F)] = \<top>" apply simp done     (* K Schema *)
+lemma a32_2_P: "[\<^bold>\<box>\<phi>\<^sup>P \<^bold>\<rightarrow> \<phi>\<^sup>P] = \<top>" apply simp done                           (* T Schema *)
+lemma a32_2_F: "[\<^bold>\<box>\<phi>\<^sup>F \<^bold>\<rightarrow> \<phi>\<^sup>F] = \<top>" apply simp done                           (* T Schema *)
 
- lemma a32_3_P: "[\<^bold>\<box>\<^bold>\<diamond>\<phi>\<^sup>P \<^bold>\<rightarrow> \<^bold>\<diamond>\<phi>\<^sup>P] = \<top>" apply simp done                       (* 5 Schema *)
- lemma a32_3_F: "[\<^bold>\<box>\<^bold>\<diamond>\<phi>\<^sup>F \<^bold>\<rightarrow> \<^bold>\<diamond>\<phi>\<^sup>F] = \<top>" apply simp done                       (* 5 Schema *)
- lemma a32_4_P: "[(\<^bold>\<forall>x. \<^bold>\<box>\<phi>\<^sup>P) \<^bold>\<rightarrow> \<^bold>\<box>((\<^bold>\<forall>x. \<phi>\<^sup>P))] = \<top>" apply simp done         (* BF *)
- lemma a32_4_F: "[(\<^bold>\<forall>x. \<^bold>\<box>\<phi>\<^sup>F) \<^bold>\<rightarrow> \<^bold>\<box>((\<^bold>\<forall>x. \<phi>\<^sup>F))] = \<top>" apply simp done         (* BF *)
+lemma a32_3_P: "[\<^bold>\<box>\<^bold>\<diamond>\<phi>\<^sup>P \<^bold>\<rightarrow> \<^bold>\<diamond>\<phi>\<^sup>P] = \<top>" apply simp done                       (* 5 Schema *)
+lemma a32_3_F: "[\<^bold>\<box>\<^bold>\<diamond>\<phi>\<^sup>F \<^bold>\<rightarrow> \<^bold>\<diamond>\<phi>\<^sup>F] = \<top>" apply simp done                       (* 5 Schema *)
+lemma a32_4_P: "[(\<^bold>\<forall>x. \<^bold>\<box>\<phi>\<^sup>P) \<^bold>\<rightarrow> \<^bold>\<box>((\<^bold>\<forall>x. \<phi>\<^sup>P))] = \<top>" apply simp done         (* BF *)
+lemma a32_4_F: "[(\<^bold>\<forall>x. \<^bold>\<box>\<phi>\<^sup>F) \<^bold>\<rightarrow> \<^bold>\<box>((\<^bold>\<forall>x. \<phi>\<^sup>F))] = \<top>" apply simp done         (* BF *)
 
-  text {* 
-  The following needs to be an axiom; it does not follow for free: it is possible that there 
-  are contingently concrete individuals and it is possible that there are not: 
-  *}
+ text {* The following needs to be an axiom; it does not follow for free: it is possible that there 
+are contingently concrete individuals and it is possible that there are not: *}
 
- axiomatization where
-   a32_5_P: "[\<^bold>\<diamond>(\<^bold>\<exists>x. \<lparr>E\<^sup>T,x\<^sup>T\<rparr> \<^bold>\<and> \<^bold>\<diamond>(\<^bold>\<not>\<lparr>E\<^sup>T,x\<^sup>T\<rparr>)) \<^bold>\<and> \<^bold>\<diamond>(\<^bold>\<not>(\<^bold>\<exists>x. \<lparr>E\<^sup>T,x\<^sup>T\<rparr> \<^bold>\<and> \<^bold>\<diamond>(\<^bold>\<not>\<lparr>E\<^sup>T,x\<^sup>T\<rparr>)))] = \<top>"
+axiomatization where
+  a32_5_P: "[\<^bold>\<diamond>(\<^bold>\<exists>x. \<lparr>E\<^sup>T,x\<^sup>T\<rparr> \<^bold>\<and> \<^bold>\<diamond>(\<^bold>\<not>\<lparr>E\<^sup>T,x\<^sup>T\<rparr>)) \<^bold>\<and> \<^bold>\<diamond>(\<^bold>\<not>(\<^bold>\<exists>x. \<lparr>E\<^sup>T,x\<^sup>T\<rparr> \<^bold>\<and> \<^bold>\<diamond>(\<^bold>\<not>\<lparr>E\<^sup>T,x\<^sup>T\<rparr>)))] = \<top>"
 
-   text {* 
-   A brief check that this axiom is well-formed, i.e. does not return error 
-   *}
- 
- lemma "[\<^bold>\<diamond>(\<^bold>\<exists>x. \<lparr>E\<^sup>T,x\<^sup>T\<rparr> \<^bold>\<and> \<^bold>\<diamond>(\<^bold>\<not>\<lparr>E\<^sup>T,x\<^sup>T\<rparr>)) \<^bold>\<and> \<^bold>\<diamond>(\<^bold>\<not>(\<^bold>\<exists>x. \<lparr>E\<^sup>T,x\<^sup>T\<rparr> \<^bold>\<and> \<^bold>\<diamond>(\<^bold>\<not>\<lparr>E\<^sup>T,x\<^sup>T\<rparr>)))] \<noteq> *" apply simp done
+  text {* A brief check that this axiom is well-formed, i.e. does not return error *}
+lemma "[\<^bold>\<diamond>(\<^bold>\<exists>x. \<lparr>E\<^sup>T,x\<^sup>T\<rparr> \<^bold>\<and> \<^bold>\<diamond>(\<^bold>\<not>\<lparr>E\<^sup>T,x\<^sup>T\<rparr>)) \<^bold>\<and> \<^bold>\<diamond>(\<^bold>\<not>(\<^bold>\<exists>x. \<lparr>E\<^sup>T,x\<^sup>T\<rparr> \<^bold>\<and> \<^bold>\<diamond>(\<^bold>\<not>\<lparr>E\<^sup>T,x\<^sup>T\<rparr>)))] \<noteq> *" apply simp done
 
+subsection {* Axioms of Necessity and Actuality *}
 
- subsection {* Axioms of Necessity and Actuality *}
-
- lemma a33_1_P: "[\<^bold>\<A>(\<phi>\<^sup>P) \<^bold>\<rightarrow> \<^bold>\<box>\<^bold>\<A>(\<phi>\<^sup>P)] = \<top>" apply simp done
- lemma a33_1_F: "[\<^bold>\<A>(\<phi>\<^sup>F) \<^bold>\<rightarrow> \<^bold>\<box>\<^bold>\<A>(\<phi>\<^sup>F)] = \<top>" apply simp done
- lemma a33_2_P: "[\<^bold>\<box>\<phi>\<^sup>P \<^bold>\<equiv> \<^bold>\<A>(\<^bold>\<box>\<phi>\<^sup>P)] = \<top>" apply simp done
- lemma a33_2_F: "[\<^bold>\<box>\<phi>\<^sup>F \<^bold>\<equiv> \<^bold>\<A>(\<^bold>\<box>\<phi>\<^sup>F)] = \<top>" apply simp done
+lemma a33_1_P: "[\<A>(\<phi>\<^sup>P) \<^bold>\<rightarrow> \<^bold>\<box>\<A>(\<phi>\<^sup>P)] = \<top>" apply simp done
+lemma a33_1_F: "[\<A>(\<phi>\<^sup>F) \<^bold>\<rightarrow> \<^bold>\<box>\<A>(\<phi>\<^sup>F)] = \<top>" apply simp done
+lemma a33_2_P: "[\<^bold>\<box>\<phi>\<^sup>P \<^bold>\<equiv> \<A>(\<^bold>\<box>\<phi>\<^sup>P)] = \<top>" apply simp done
+lemma a33_2_F: "[\<^bold>\<box>\<phi>\<^sup>F \<^bold>\<equiv> \<A>(\<^bold>\<box>\<phi>\<^sup>F)] = \<top>" apply simp done
 
 
- subsection {* Axioms for Descriptions *}
+subsection {* Axioms for Descriptions *}
 
-  text {* 
-  ... here I still run into some problems, need to analyze why both
-  formulas result in errors, check carefully again definition of equality and description ... 
-  *}
-
- lemma a34_Inst_1: "[(x\<^sup>T \<^bold>= (\<^bold>\<iota> x. \<lparr>R\<^sup>T,x\<^sup>T\<rparr>)) \<^bold>\<equiv> (\<^bold>\<forall> z. (\<^bold>\<A>\<lparr>R\<^sup>T,z\<^sup>T\<rparr> \<^bold>\<equiv> (z\<^sup>T \<^bold>= x\<^sup>T)))] = *" apply simp done
- lemma a34_Inst_2: "[(x\<^sup>T \<^bold>= (\<^bold>\<iota> x. (\<phi>(x))\<^sup>T)) \<^bold>\<equiv> (\<^bold>\<forall> z. (\<^bold>\<A>((\<phi>(z))\<^sup>T) \<^bold>\<equiv> (z\<^sup>T \<^bold>= x\<^sup>T)))] = *" apply simp done
-
- (*
- lemma a34_Inst_test1: "(x\<^sup>T \<^bold>= (\<^bold>\<iota> x. \<lparr>R\<^sup>T,x\<^sup>T\<rparr>)) = X" apply simp oops
- lemma a34_Inst_test2: "(\<^bold>\<forall> z. (\<^bold>\<A>\<lparr>R\<^sup>T,z\<^sup>T\<rparr> \<^bold>\<equiv> (z\<^sup>T \<^bold>= x\<^sup>T))) = X" apply simp oops
- *)
+ text {* ... here I still run into some problems, need to analyze why both
+ formulas result in errors, check carefully again definition of equality and description ... *}
 
 
-(*<*)
-section {* Various Test Examples *}
+lemma a34_Inst_1: "[(x\<^sup>T \<^bold>= (\<iota> x. \<lparr>R\<^sup>T,x\<^sup>T\<rparr>)) \<^bold>\<equiv> (\<^bold>\<forall> z. (\<A>\<lparr>R\<^sup>T,z\<^sup>T\<rparr> \<^bold>\<equiv> (z\<^sup>T \<^bold>= x\<^sup>T)))] = *" apply simp done
+lemma a34_Inst_2: "[(x\<^sup>T \<^bold>= (\<iota> x. (\<phi>(x))\<^sup>T)) \<^bold>\<equiv> (\<^bold>\<forall> z. (\<A>((\<phi>(z))\<^sup>T) \<^bold>\<equiv> (z\<^sup>T \<^bold>= x\<^sup>T)))] = *" apply simp done
 
-  text {* Todo: ... select, adapt, and explain some of examples below ... *}
-
- lemma "\<lparr>\<^bold>\<lambda>x. \<lparr>R\<^sup>T,x\<^sup>T\<rparr> \<^bold>\<rightarrow> \<lbrace>x\<^sup>T,R\<^sup>T\<rbrace>,a\<^sup>T\<rparr> = X" apply simp oops
-
- lemma "\<exists>X. \<lparr>\<^bold>\<lambda>x. \<lparr>R\<^sup>T,x\<^sup>T\<rparr> \<^bold>\<rightarrow> \<lparr>R\<^sup>T,x\<^sup>T\<rparr>,a\<^sup>T\<rparr> = X\<^sup>P" apply simp done -- {* Solution: @{text "(\<lambda>w. True) = X"} *}
- lemma "[\<lparr>\<^bold>\<lambda>x. \<lparr>R\<^sup>T,x\<^sup>T\<rparr> \<^bold>\<rightarrow> \<lparr>R\<^sup>T,x\<^sup>T\<rparr>,a\<^sup>T\<rparr>] = \<top>" apply simp done
-
- lemma "\<lparr>\<^bold>\<lambda>x. \<lparr>R\<^sup>T,x\<^sup>T\<rparr> \<^bold>\<rightarrow> \<lparr>R\<^sup>T,x\<^sup>T\<rparr>,a\<^sup>T\<rparr> = X\<^sup>P" apply simp oops
- lemma "(\<^bold>\<lambda>x. \<lparr>R\<^sup>T,x\<^sup>T\<rparr> \<^bold>\<rightarrow> \<lbrace>x\<^sup>T,R\<^sup>T\<rbrace>) = X" apply simp oops
-
- lemma "[(\<^bold>\<forall>x. \<lparr>R\<^sup>T,x\<^sup>T\<rparr> \<^bold>\<rightarrow> \<lparr>R\<^sup>T,x\<^sup>T\<rparr>)] = \<top>" apply simp done
- lemma "[(\<^bold>\<forall>R. \<^bold>\<forall>(\<lambda>x. \<lparr>R\<^sup>T,x\<^sup>T\<rparr> \<^bold>\<rightarrow> \<lparr>R\<^sup>T,x\<^sup>T\<rparr>))] = \<top>" apply simp done
- lemma "(\<^bold>\<forall>x. \<lparr>R\<^sup>T,x\<^sup>T\<rparr> \<^bold>\<rightarrow> \<lparr>R\<^sup>T,x\<^sup>T\<rparr>) = X" apply simp oops
-
- lemma "[(\<^bold>\<forall>x. \<lbrace>x\<^sup>T,R\<^sup>T\<rbrace> \<^bold>\<rightarrow> \<lbrace>x\<^sup>T,R\<^sup>T\<rbrace>)] = \<top>" apply simp done
- lemma "(\<^bold>\<forall>x. \<lbrace>x\<^sup>T,R\<^sup>T\<rbrace> \<^bold>\<rightarrow> \<lbrace>x\<^sup>T,R\<^sup>T\<rbrace>) = X" apply simp oops
-
- lemma "[(\<^bold>\<exists>x y. \<lbrace>x\<^sup>T,R\<^sup>T\<rbrace> \<^bold>\<rightarrow> \<lbrace>y\<^sup>T,R\<^sup>T\<rbrace>)] = \<top>" apply simp done
-
- lemma "[(\<^bold>\<forall>x. \<lparr>R\<^sup>T,x\<^sup>T\<rparr> \<^bold>\<rightarrow> \<lbrace>x\<^sup>T,R\<^sup>T\<rbrace>)] = *" apply simp done
- lemma "[(\<^bold>\<forall>x. \<lparr>R\<^sup>T,x\<^sup>T\<rparr> \<^bold>\<rightarrow> \<lbrace>x\<^sup>T,R\<^sup>T\<rbrace>)] = X" apply simp oops
- lemma "(\<^bold>\<forall>x. \<lparr>R\<^sup>T,x\<^sup>T\<rparr> \<^bold>\<rightarrow> \<lbrace>x\<^sup>T,R\<^sup>T\<rbrace>) = X" apply simp oops
- lemma "[(\<^bold>\<forall>R. \<lparr>R\<^sup>T,x\<^sup>T\<rparr> \<^bold>\<rightarrow> \<lbrace>x\<^sup>T,R\<^sup>T\<rbrace>)] = *" apply simp done
- lemma "(\<^bold>\<forall>R. \<lparr>R\<^sup>T,x\<^sup>T\<rparr> \<^bold>\<rightarrow> \<lbrace>x\<^sup>T,R\<^sup>T\<rbrace>) = X" apply simp oops
-
- lemma "[(\<^bold>\<forall>x. \<^bold>\<exists>(\<lambda>R. \<lbrace>x\<^sup>T,R\<^sup>T\<rbrace> \<^bold>\<rightarrow> \<lbrace>x\<^sup>T,R\<^sup>T\<rbrace>))] = \<top>" apply simp done
- lemma "[(\<^bold>\<exists>x. \<^bold>\<forall>(\<lambda>R. \<lbrace>x\<^sup>T,R\<^sup>T\<rbrace> \<^bold>\<rightarrow> \<lbrace>x\<^sup>T,R\<^sup>T\<rbrace>))] = \<top>" apply simp done
-(*>*)
+(*
+lemma a34_Inst_test1: "(x\<^sup>T \<^bold>= (\<iota> x. \<lparr>R\<^sup>T,x\<^sup>T\<rparr>)) = X" apply simp oops
+lemma a34_Inst_test2: "(\<^bold>\<forall> z. (\<A>\<lparr>R\<^sup>T,z\<^sup>T\<rparr> \<^bold>\<equiv> (z\<^sup>T \<^bold>= x\<^sup>T))) = X" apply simp oops
+*)
 
 (*<*)
 end
